Clean up commented out code.  Add model check level indexed step relation and running time bound

protocols/PartialOrderReduction.v
@@ -18,6 +18,7 @@
 
 From Coq Require Import
      Classical
+     Morphisms
      List.
 
 From KeyManagement Require Import
@@ -1112,13 +1113,7 @@ Section RealWorldLemmas.
     simpl; rewrite H24; eauto.
   Qed.
 
-  (* rather than just running last user, need some computation that finds next available person to run 
-   * 
-   * does this really do what I want it to?
-   *)
-
-
-  Lemma has_user_step {A B} (U : universe A B) (u_id : user_id) :
+  Lemma user_step_or_not {A B} (U : universe A B) (u_id : user_id) :
     forall u_d,
       U.(users) $? u_id = Some u_d
       -> (exists lbl U', step_user lbl (Some u_id) (build_data_step U u_d) U')
@@ -1138,21 +1133,6 @@ Section RealWorldLemmas.
       destruct x; eauto.
       apply NNPP in H0; eauto.
   Qed.
-
-  (* Inductive nextStep {A B} (U : universe A B) : *)
-  (*   forall (usrs : list (user_id * user_data A)), (forall uid ud, List.In (uid,ud) usrs -> U.(users) $? uid = Some ud) -> Prop := *)
-
-  (* | Here : forall us us' mapIn lbl bd' u_id userData, *)
-  (*     us = (u_id,userData) :: us' *)
-  (*     -> step_user lbl (Some u_id) (build_data_step U userData) bd' *)
-  (*     -> nextStep U us mapIn *)
-
-  (* | There : forall us us' mapIn mapIn' u_id userData, *)
-  (*     us = (u_id,userData) :: us' *)
-  (*     -> (forall lbl bd', ~ step_user lbl (Some u_id) (build_data_step U userData) bd') *)
-  (*     -> nextStep U us' mapIn' *)
-  (*     -> nextStep U us mapIn *)
-  (* . *)
 
   Definition summarize_univ {A B} (U : universe A B) (summaries : NatMap.t summary) : Prop :=
     forall u_id u_d s,
@@ -1213,37 +1193,6 @@ Section RealWorldLemmas.
                                                    sent_nons := sents;
                                                    cur_nonce := cur_n; |}
       -> step_universeC U lbl U'. 
-
-  (* Definition universeStepCommutes {A B} (U U' : universe A B) : Prop := *)
-  (*   forall lbl1 lbl2 U'' u_id1 u_id2 ud1 ud2 bd1 bd2 summaries, *)
-  (*     step_universe U lbl1 U' *)
-  (*     -> step_universe U' lbl2 U'' *)
-  (*     -> U.(users) $? u_id1 = Some ud1 *)
-  (*     -> step_user lbl1 (Some u_id1) (build_data_step U ud1) bd1 *)
-  (*     -> U'.(users) $? u_id2 = Some ud2 *)
-  (*     -> step_user lbl2 (Some u_id2) (build_data_step U' ud2) bd2 *)
-  (*     -> u_id1 <> u_id2 *)
-  (*     -> summarize_univ U summaries *)
-  (*     -> (forall C (cmd__n : user_cmd C) s, *)
-  (*         nextAction ud2.(protocol) cmd__n *)
-  (*         -> forall uid ud, *)
-  (*           uid <> u_id2 *)
-  (*           -> U.(users) $? uid = Some ud *)
-  (*           -> summarize ud.(protocol) s *)
-  (*           -> commutes cmd__n s) *)
-  (*     -> True. *)
-
-  (* Lemma commutes_sound_universe : *)
-  (*   forall {A B} (U U' U'' : universe A B) lbl1 lbl2, *)
-  (*     step_universe U lbl1 U' *)
-  (*     -> step_universe U' lbl2 U'' *)
-  (*     -> universeStepCommutes U U' *)
-  (*     -> exists U''' lbl3 lbl4, *)
-  (*         step_user lbl3 (Some u_id2) (build_data_step U__r userData2) bd3 *)
-  (*             /\ U__r'' = buildUniverse_step bd3 u_id2 *)
-  (*             /\ U__r''.(users) $? u_id1 = Some userData1' *)
-  (*             /\ step_user lbl4 (Some u_id1) (build_data_step U__r'' userData1') bd3' *)
-  (*             /\ buildUniverse_step bd3' u_id1 = buildUniverse_step bd1' u_id2 *)
 
   Lemma silent_step_nochange_other_user' :
     forall {A B C} suid lbl bd bd',
@@ -1437,61 +1386,6 @@ Section RealWorldLemmas.
     intros; subst; eapply step_limited_change_other_user'; eauto.
   Qed.
 
-  (* Lemma step_limited_change_other_user_func' : *)
-  (*   forall {A B C} suid lbl bd bd', *)
-  (*     step_user lbl suid bd bd' *)
-  (*     -> forall cs cs' (usrs usrs': honest_users A) (adv adv' : user_data B) gks gks' *)
-  (*         (cmd cmd' : user_cmd C) ks ks' qmsgs qmsgs' mycs mycs' *)
-  (*         froms froms' sents sents' cur_n cur_n', *)
-  (*       bd = (usrs, adv, cs, gks, ks, qmsgs, mycs, froms, sents, cur_n, cmd) *)
-  (*       -> bd' = (usrs', adv', cs', gks', ks', qmsgs', mycs', froms', sents', cur_n', cmd') *)
-  (*       -> forall cmdc cmdc' u_id1, *)
-  (*           suid = Some u_id1 *)
-  (*           -> usrs $? u_id1 = Some {| key_heap := ks; *)
-  (*                                     protocol := cmdc; *)
-  (*                                     msg_heap := qmsgs; *)
-  (*                                     c_heap   := mycs; *)
-  (*                                     from_nons := froms; *)
-  (*                                     sent_nons := sents; *)
-  (*                                     cur_nonce := cur_n |} *)
-  (*           -> (forall uid u, *)
-  (*                 usrs $? uid = Some u *)
-  (*                 ->  *)
-
-
-  (*           -> ( usrs'' $? u_id2 = Some {| key_heap := ks2; *)
-  (*                                         protocol := cmdc2; *)
-  (*                                         msg_heap := qmsgs2; *)
-  (*                                         c_heap   := mycs2; *)
-  (*                                         from_nons := froms2; *)
-  (*                                         sent_nons := sents2; *)
-  (*                                         cur_nonce := cur_n2 |} *)
-  (*             \/ exists m, *)
-  (*               usrs'' $? u_id2 = Some {| key_heap := ks2; *)
-  (*                                         protocol := cmdc2; *)
-  (*                                         msg_heap := qmsgs2 ++ [m]; *)
-  (*                                         c_heap   := mycs2; *)
-  (*                                         from_nons := froms2; *)
-  (*                                         sent_nons := sents2; *)
-  (*                                         cur_nonce := cur_n2 |} ) *)
-  (* . *)
-  (* Proof. *)
-  (*   induction 1; inversion 1; inversion 1; *)
-  (*     intros; subst; *)
-  (*       try solve [ split; [intros | left; clean_map_lookups; trivial]; eauto ]. *)
-    
-  (*   - specialize (IHstep_user _ _ _ _ _ _ _ _ _ _ _ *)
-  (*                             _ _ _ _ _ _ _ _ _ _ _ *)
-  (*                             eq_refl eq_refl). *)
-  (*     specialize (IHstep_user cmdc cmdc'). *)
-  (*     specialize (IHstep_user _ _ _ _ _ _ _ _ _ _ eq_refl H25 H26 H27 eq_refl). *)
-  (*     split_ors; eauto. *)
-
-  (*   - split; [ | clean_context; clean_map_lookups]; eauto. *)
-  (*     destruct (rec_u_id ==n u_id2); subst; eauto. *)
-  (* Qed. *)
-  
-
 End RealWorldLemmas.
 
 Section AuxDefinitions.
@@ -1527,8 +1421,6 @@ Section AuxDefinitions.
 
   Hint Extern 1 (_ < _) => Omega.omega : core.
   Hint Extern 1 (_ <= _) => Omega.omega : core.
-
-  From Coq Require Import Morphisms.
 
   Definition queues_size {A} (usrs : honest_users A) : nat :=
     fold (fun uid ud acc => acc + length ud.(msg_heap)) usrs 0.
@@ -1707,50 +1599,6 @@ Section AuxDefinitions.
 
   Hint Constructors boundRunningTimeUniv : core.
 
-  (* Lemma boundRunningTime_for_element' : *)
-  (*   forall A (usrs : list (user_id * user_data A)) n__rt, *)
-  (*     boundRunningTimeUniv usrs n__rt *)
-  (*     -> forall uid u, *)
-  (*       List.In (uid,u) usrs *)
-  (*       -> exists n, *)
-  (*         boundRunningTime u.(protocol) n. *)
-  (* Proof. *)
-  (*   induction usrs; intros; simpl in *; try contradiction. *)
-  (*   invert H. *)
-  (*   split_ors; eauto. *)
-  (*   invert H; eauto. *)
-  (* Qed. *)
-
-  (* Lemma ina_in : *)
-  (*   forall X Y (x : X) (y : Y) (l : list (X * Y)), *)
-  (*     SetoidList.InA (fun p p' : X * Y => fst p = fst p' /\ snd p = snd p') (x,y) l *)
-  (*     -> List.In (x,y) l. *)
-  (* Proof. *)
-  (*   induction 1; simpl in *; eauto. *)
-  (*   destruct y0;  *)
-  (*     split_ands; subst; eauto. *)
-  (* Qed. *)
-
-  (* Lemma in_ina : *)
-  (*   forall X Y (x : X) (y : Y) (l : list (X * Y)), *)
-  (*     List.In (x,y) l *)
-  (*     -> SetoidList.InA (fun p p' : X * Y => fst p = fst p' /\ snd p = snd p') (x,y) l. *)
-  (* Proof. *)
-  (*   induction l; intros; simpl in *; try contradiction; eauto. *)
-  (*   split_ors; subst; eauto. *)
-  (* Qed. *)
-
-  (* Lemma eqlistA_eq : *)
-  (*   forall Y n (y : Y) (m : NatMap.t Y), *)
-  (*     SetoidList.eqlistA *)
-  (*       (fun p p' : nat * Y => fst p = fst p' /\ snd p = snd p') (elements (m $+ (n, y))) *)
-  (*       (O.elements_lt (n,y) m ++ (n,y) :: O.elements_ge (n,y) m) *)
-  (*     -> elements (m $+ (n,y)) = O.elements_lt (n,y) m ++ (n,y) :: O.elements_ge (n,y) m. *)
-  (* Proof. *)
-  (*   induction 1; simpl in *; subst; eauto. *)
-  (*   destruct x; destruct x'; simpl in *; split_ands; subst; trivial. *)
-  (* Qed. *)
-
   Lemma boundRunningTime_for_element :
     forall A (usrs : honest_users A) n__rt,
       boundRunningTimeUniv usrs n__rt
@@ -1792,164 +1640,6 @@ Section AuxDefinitions.
       destruct (y ==n uid); destruct (y ==n uid0); subst; clean_map_lookups; eauto.
       rewrite RW; auto.
   Qed.
-
-  (* Lemma boundRunningTimeUniv_split' : *)
-  (*   forall A (usrs : list (user_id * user_data A)) n__rt, *)
-  (*     boundRunningTimeUniv usrs n__rt *)
-  (*     -> forall usrs1 usrs2 uid u, *)
-  (*       usrs = usrs1 ++ (uid,u) :: usrs2 *)
-  (*       -> exists n, *)
-  (*         boundRunningTime u.(protocol) n *)
-  (*       /\ n <= n__rt *)
-  (*       /\ boundRunningTimeUniv (usrs1 ++ usrs2) (n__rt - n). *)
-  (* Proof. *)
-  (*   induction usrs; intros; simpl in *; try discriminate. *)
-  (*   - destruct usrs1. *)
-  (*     rewrite app_nil_l in H0; invert H0. *)
-  (*     rewrite <- app_comm_cons in H0; invert H0. *)
-
-  (*   - invert H. *)
-  (*     specialize (IHusrs _ H5). *)
-  (*     destruct usrs1. *)
-  (*     * rewrite app_nil_l in *. *)
-  (*       invert H0. *)
-  (*       destruct usrs2. *)
-  (*       ** invert H5. *)
-  (*          eexists; rewrite plus_0_r; repeat simple apply conj; eauto. *)
-  (*          rewrite Nat.sub_diag; eauto. *)
-  (*       ** invert H5. *)
-  (*          specialize (IHusrs [] usrs2 uid0 u0). *)
-  (*          rewrite app_nil_l in IHusrs. *)
-  (*          specialize (IHusrs eq_refl); split_ex. *)
-  (*          eexists; repeat simple apply conj; eauto. *)
-
-  (*          rewrite Nat.add_comm. *)
-  (*          rewrite <- Nat.add_assoc. *)
-  (*          rewrite <- Nat.add_sub_assoc; eauto. *)
-
-  (*          econstructor; eauto. *)
-  (*          rewrite <- Nat.add_sub_assoc; eauto. *)
-  (*          rewrite Nat.sub_diag. *)
-  (*          rewrite plus_0_r; eauto. *)
-
-  (*     * rewrite <- app_comm_cons in *. *)
-  (*       invert H0. *)
-  (*       specialize (IHusrs usrs1 usrs2 uid u eq_refl); split_ex. *)
-  (*       eexists; repeat simple apply conj; eauto. *)
-  (*       rewrite <- Nat.add_sub_assoc; eauto. *)
-  (* Qed. *)
-
-  (* Lemma map_remove_add_eq : *)
-  (*   forall {V} (m : Map.t V) k v, *)
-  (*     m $- k $+ (k, v) = m $+ (k, v). *)
-  (* Proof. *)
-  (*   intros. apply map_eq_Equal; unfold Equal; intros. *)
-  (*   destruct (k ==n y); subst; clean_map_lookups; auto. *)
-  (* Qed. *)
-
-  (* Lemma update_map_list' : *)
-  (*   forall V (m : NatMap.t V) k v, *)
-  (*     m $? k = Some v *)
-  (*     -> exists usrs1 usrs2, *)
-  (*       elements m = usrs1 ++ (k,v) :: usrs2 *)
-  (*     /\ usrs1 = O.elements_lt (k,v) (m $- k) *)
-  (*     /\ usrs2 = O.elements_ge (k,v) (m $- k) *)
-  (*     /\ (forall v', ~ List.In (k,v') usrs2). *)
-  (* Proof. *)
-  (*   intros. *)
-
-  (*   assert (ADD: Add k v (m $- k) (m $- k $+ (k,v))). *)
-  (*   unfold Add; intros; destruct (y ==n k); subst; clean_map_lookups; trivial. *)
-
-  (*   apply O.elements_Add in ADD; eauto. *)
-  (*   apply eqlistA_eq in ADD; eauto. *)
-
-  (*   assert (RW : m $- k $+ (k,v) = m). *)
-  (*   apply map_eq_Equal; unfold Equal; intros; destruct (y ==n k); subst; clean_map_lookups; auto. *)
-
-  (*   rewrite RW in *. *)
-  (*   exists (O.elements_lt (k, v) (m $- k)). *)
-  (*   exists (O.elements_ge (k, v) (m $- k)). *)
-  (*   repeat simple apply conj; eauto. *)
-
-  (*   unfold not; intros. *)
-  (*   unfold O.elements_ge in H0. *)
-  (*   rewrite filter_In in H0; split_ands. *)
-  (*   apply in_ina in H0. *)
-  (*   rewrite <- elements_mapsto_iff in H0. *)
-  (*   rewrite remove_mapsto_iff in H0; split_ands; contradiction. *)
-  (* Qed. *)
-
-  (* Lemma elements_lt_val_nomatter' : *)
-  (*   forall V (l : list (nat * V)) k v v', *)
-  (*     List.filter (O.gtb (k, v)) l = List.filter (O.gtb (k, v')) l. *)
-  (* Proof. *)
-  (*   induction l; eauto. *)
-  (* Qed. *)
-
-  (* Lemma elements_lt_val_nomatter : *)
-  (*   forall V (m : NatMap.t V) k v v', *)
-  (*     O.elements_lt (k,v) m = O.elements_lt (k,v') m. *)
-  (* Proof. *)
-  (*   intros; eauto using elements_lt_val_nomatter'. *)
-  (* Qed. *)
-  
-  (* Lemma update_map_list : *)
-  (*   forall V (m : NatMap.t V) k v v', *)
-  (*     m $? k = Some v *)
-  (*     -> exists usrs1 usrs2, *)
-  (*       elements m = usrs1 ++ (k,v) :: usrs2 *)
-  (*     /\ elements (m $+ (k,v')) = usrs1 ++ (k,v') :: usrs2. *)
-  (* Proof. *)
-  (*   intros; subst. *)
-  (*   assert (M' : m $+ (k,v') $? k = Some v') by (clean_map_lookups; trivial). *)
-
-  (*   generalize (update_map_list' _ _ H); intros; split_ex; subst. *)
-  (*   generalize (update_map_list' _ _ M'); intros; split_ex; subst. *)
-  (*   rewrite !map_add_remove_eq in H1. *)
-  (*   rewrite !elements_lt_val_nomatter with (v := v') (v' := v) in H1; eauto. *)
-  (* Qed. *)
-
-  (* Lemma boundRunningTimeUniv_app : *)
-  (*   forall A (l1 l2 : list (nat * user_data A)) n, *)
-  (*     boundRunningTimeUniv (l1 ++ l2) n *)
-  (*     -> exists n1 n2, *)
-  (*       boundRunningTimeUniv l1 n1 *)
-  (*     /\ boundRunningTimeUniv l2 n2 *)
-  (*     /\ n = n1 + n2. *)
-  (* Proof. *)
-  (*   induction l1; intros; eauto. *)
-  (*   rewrite <- app_comm_cons in H. *)
-  (*   invert H. *)
-  (*   specialize (IHl1 _ _ H4); split_ex. *)
-  (*   (do 2 eexists); repeat simple apply conj; eauto. *)
-  (*   Omega.omega. *)
-  (* Qed. *)
-
-  (* Lemma listIn_iff_false : *)
-  (*   forall A (usrs : list (nat * user_data A)), *)
-  (*     (forall uid ud, List.In (uid,ud) usrs <-> False) *)
-  (*     -> usrs = []. *)
-  (* Proof. *)
-  (*   induction usrs; intros; eauto. *)
-  (*   exfalso. *)
-  (*   destruct a. *)
-  (*   specialize (H n u). *)
-  (*   destruct H; eauto. *)
-  (* Qed. *)
-
-  (* Lemma listIn_false : *)
-  (*   forall A (usrs : list (nat * user_data A)), *)
-  (*     (forall uid ud, List.In (uid,ud) usrs -> exists (ud : user_data A), False) *)
-  (*     -> usrs = []. *)
-  (* Proof. *)
-  (*   induction usrs; intros; eauto. *)
-  (*   exfalso. *)
-  (*   destruct a. *)
-  (*   specialize (H n u); eauto. *)
-  (*   assert (IN : List.In (n,u) ((n,u)::usrs)) by eauto. *)
-  (*   specialize (H IN); split_ex; contradiction. *)
-  (* Qed. *)
 
   Lemma map_no_entries_empty :
     forall A (usrs : honest_users A),
@@ -2002,28 +1692,6 @@ Section AuxDefinitions.
       
       eexists; split; eauto.
   Qed.
-
-  (* Definition appendMsg {A} (ud : user_data A) (m : {x : type & crypto x} ) := *)
-  (*   {| key_heap := ud.(key_heap); *)
-  (*      protocol := ud.(protocol); *)
-  (*      msg_heap := ud.(msg_heap) ++ [m]; *)
-  (*      c_heap   := ud.(c_heap); *)
-  (*      from_nons := ud.(from_nons); *)
-  (*      sent_nons := ud.(sent_nons); *)
-  (*      cur_nonce := ud.(cur_nonce) |}. *)
-
-  (* Lemma boundedRunningTimeUniv_generalize : *)
-  (*   forall A (usrs : list (nat * user_data A)) n, *)
-  (*     boundRunningTimeUniv usrs n *)
-  (*     -> forall (f : user_data A -> user_data A) usrs', *)
-  (*       (forall ud, (f ud).(protocol) = ud.(protocol)) *)
-  (*       -> usrs' = List.map (fun '(uid,u) => (uid, f u)) usrs *)
-  (*       -> boundRunningTimeUniv usrs' n. *)
-  (* Proof. *)
-  (*   induction 1; intros; subst; simpl; eauto. *)
-  (*   econstructor; eauto. *)
-  (*   rewrite (H1 u); eauto. *)
-  (* Qed. *)
 
   Lemma user_step_removes_no_users_keeps_proto :
     forall {A B C} cs cs' lbl u_id (usrs usrs' : honest_users A) (adv adv' : user_data B)
@@ -2111,99 +1779,6 @@ Section AuxDefinitions.
       rewrite remove_neq_o in * by congruence; eauto.
   Qed.
 
-    
-  (* Lemma boundRunningTime_univ_update : *)
-  (*   forall A (usrs : honest_users A) n__rt, *)
-  (*     boundRunningTimeUniv (elements usrs) n__rt *)
-  (*     -> forall uid u1 u2 p1 p2 n1 n2, *)
-  (*       usrs $? uid = Some u1 *)
-  (*       -> p1 = u1.(protocol) *)
-  (*       -> p2 = u2.(protocol) *)
-  (*       -> boundRunningTime p1 n1 *)
-  (*       -> boundRunningTime p2 n2 *)
-  (*       -> boundRunningTimeUniv (elements (usrs $+ (uid,u2))) (n__rt + n2 - n1). *)
-  (* Proof. *)
-  (*   intros. *)
-    
-  (* Admitted. *)
-
-  (*   H2 : boundRunningTimeUniv (elements (elt:=user_data A) (users U)) n__rt *)
-  (* H3 : queues_size (users U) = n__qs *)
-  (* x : nat *)
-  (* H4 : boundRunningTime protocol x *)
-  (* STEP : step_user lbl (Some u_id) *)
-  (*          (users U, adversary U, all_ciphers U, all_keys U, key_heap, msg_heap, c_heap, from_nons, sent_nons, *)
-  (*          cur_nonce, protocol) (usrs, adv, cs, gks, ks, qmsgs, mycs, froms, sents, cur_n, cmd) *)
-  (* x0 : nat *)
-  (* H1 : boundRunningTime cmd x0 *)
-
-  (* Lemma boundRunningTimeUniv_step' : *)
-  (*   forall A B cs cs' (usrs usrs': honest_users A) (adv adv' : user_data B) gks gks' *)
-  (*     (cmd' : user_cmd C) ks ks' qmsgs qmsgs' mycs mycs' *)
-  (*     froms froms' sents sents' cur_n cur_n' lbl cmda cmda' uid, *)
-        
-  (*     step_user lbl (Some uid) *)
-  (*               (usrs, adv, cs, gks, ks, qmsgs, mycs, froms, sents, cur_n, cmd) *)
-  (*               (usrs', adv', cs', gks', ks', qmsgs', mycs', froms', sents', cur_n', cmd') *)
-  (*     -> forall cmda n__rt, *)
-  (*       usrs $? uid = Some (mkUserData ks cmda qmsgs mycs froms sents cur_n) *)
-  (*       -> boundRunningTimeUniv (elements usrs) n__rt *)
-  (*       -> forall other_id other p, *)
-  (*           other_id <> uid *)
-  (*           -> usrs $? other_id = Some other *)
-  (*           ->  *)
-
-
-  (*       -> exists n', *)
-  (*         boundRunningTime cmd' n' *)
-  (*         /\ n' + queues_size (usrs' $+ (uid, mkUserData ks' cmda' qmsgs' mycs' froms' sents' cur_n' )) *)
-  (*           < n + queues_size usrs. *)
-  (* Proof. *)
-  (*   induction 1; *)
-  (*     invert 1; *)
-  (*     intros; *)
-  (*     try solve [ exists n; simpl; erewrite <- queues_size_readd_user_same_queue_idem by eauto; split; eauto ]. *)
-
-  (*   - assert (uid <> uid0) by (unfold not; intros RW; rewrite RW in *; contradiction). *)
-  (*     rewrite map_ne_swap by eauto. *)
-
-  (*     erewrite queues_size_readd_user_addnl_msg with (uid := uid). *)
-  (*     3: reflexivity. *)
-  (*     2: clean_map_lookups; reflexivity. *)
-  (*     2: simpl; reflexivity. *)
-      
-  (*     erewrite <- queues_size_readd_user_same_queue_idem by eauto. *)
-
-  (*     exists n; split; eauto. *)
-      
-  (*   - exists (n + 1); split; eauto. *)
-  (*     rewrite <- plus_assoc. *)
-  (*     erewrite <- queues_size_readd_user_popped_msg; eauto; eauto. *)
-  (*     simpl; eauto. *)
-      
-  (*   - exists (2 + n); split; eauto. *)
-
-  (*     rewrite <- plus_assoc. *)
-  (*     rewrite plus_comm with (n := n). *)
-  (*     rewrite plus_assoc. *)
-  (*     rewrite <- plus_assoc with (n := 1). *)
-  (*     erewrite <- queues_size_readd_user_popped_msg; eauto; eauto. *)
-  (*     simpl; eauto. *)
-
-  (*   - eapply IHboundRunningTime in H9; split_ex; eauto. *)
-  (*     eexists; split; eauto. *)
-  (*     rewrite plus_comm with (n := x). *)
-  (*     rewrite plus_comm with (n := n1). *)
-  (*     rewrite !plus_assoc. *)
-  (*     rewrite <- plus_assoc. *)
-  (*     rewrite <- plus_assoc with (m := n1). *)
-  (*     apply Nat.add_lt_mono_l; eauto. *)
-      
-  (*   - erewrite <- queues_size_readd_user_same_queue_idem by eauto. *)
-  (*     eexists; split; eauto. *)
-      
-  (* Qed. *)
-
   Lemma boundRunningTime_univ_step :
     forall A B (U U' : universe A B) lbl b n__rt n__qs,
       step_universe U lbl U'
@@ -2244,7 +1819,7 @@ Section AuxDefinitions.
 
   Hint Constructors runningTimeMeasure : core.
 
-  Lemma runningTimeMeasure_step :
+  Lemma runningTimeMeasure_stepU :
     forall A B (U U' : universe A B) lbl b n,
       step_universe U lbl U'
       -> lameAdv b U.(adversary)
@@ -2280,43 +1855,80 @@ Section AuxDefinitions.
     - rewrite H in H1; invert H1.
   Qed.
 
+  Lemma runningTimeMeasure_step :
+    forall A B (st st' : RealWorld.universe A B * IdealWorld.universe A) b n,
+      step st st'
+      -> lameAdv b (fst st).(adversary)
+      -> runningTimeMeasure (fst st) n
+      -> exists n',
+          runningTimeMeasure (fst st') n'
+          /\ n' < n.
+  Proof.
+    destruct st; destruct st'; simpl;
+      inversion 3; subst; eauto.
+    invert H; eauto using runningTimeMeasure_stepU.
+  Qed.
+  
   Lemma runningTimeMeasure_steps :
-    forall A B (U U' : universe A B),
-      trc3 step_universe ign_lbl U U'
+    forall A B (st st' : RealWorld.universe A B * IdealWorld.universe A),
+      (@step A B) ^* st st'
       -> forall b n,
-        lameAdv b U.(adversary)
-        -> runningTimeMeasure U n
+        lameAdv b (fst st).(adversary)
+        -> runningTimeMeasure (fst st) n
         -> exists n',
-            runningTimeMeasure U' n'
+            runningTimeMeasure (fst st') n'
           /\ n' <= n.
   Proof.
     induction 1; intros; eauto.
-    generalize H0; intros STEP.
-    eapply runningTimeMeasure_step in H0; eauto; split_ex.
+    generalize H; intros STEP.
+    eapply runningTimeMeasure_step in H; eauto; split_ex.
 
-    assert (lameAdv b0 (adversary y)).
-    eapply adversary_remains_lame; eauto.
+    assert (lameAdv b (adversary (fst y))).
+    invert STEP;
+      eapply adversary_remains_lame; eauto.
 
-    specialize (IHtrc3 _ _ H5 H0); split_ex; eauto.
+    specialize (IHtrc _ _ H4 H); split_ex; eauto.
   Qed.
 
-  Inductive stepsi {A B} :
+  Inductive rstepsi {A B} :
     nat -> universe A B  -> universe A B -> Prop :=
-  | StepsiO : forall U,
-      stepsi O U U
-  | StepsiS : forall lbl U U' U'' i,
+  | RStepsiO : forall U,
+      rstepsi O U U
+  | RStepsiS : forall lbl U U' U'' i,
       step_universe U lbl U'
-      -> stepsi i U' U''
-      -> stepsi (1 + i) U U''.
+      -> rstepsi i U' U''
+      -> rstepsi (1 + i) U U''.
 
-  Hint Constructors stepsi : core.
+  Hint Constructors rstepsi : core.
 
-  Lemma steps_stepsi :
+  Lemma rsteps_rstepsi :
     forall A B pr (U U' : universe A B),
       trc3 step_universe pr U U'
-      -> exists i, stepsi i U U'.
+      -> exists i, rstepsi i U U'.
   Proof.
-    induct 1; split_ex; eauto.
+    induction 1; split_ex; eauto.
+  Qed.
+
+  Inductive stepsi {t__hon t__adv} :
+    nat 
+  -> (RealWorld.universe t__hon t__adv * IdealWorld.universe t__hon)
+  -> (RealWorld.universe t__hon t__adv * IdealWorld.universe t__hon)
+  -> Prop :=
+  | StepsiO : forall st,
+      stepsi O st st
+  | StepsiS : forall st st' st'' i,
+      step st st' 
+      -> stepsi i st' st''
+      -> stepsi (1 + i) st st''.
+
+  Hint Constructors step stepsi : core.
+    
+  Lemma steps_stepsi :
+    forall t__hon t__adv (st st' : RealWorld.universe t__hon t__adv * IdealWorld.universe t__hon),
+      step st st'
+      -> exists i, stepsi i st st'.
+  Proof.
+    induction 1; split_ex; eauto.
   Qed.
 
 End AuxDefinitions.
